cedar-lean/Cedar/Thm.lean
@@ -26,3 +26,4 @@ import Cedar.Thm.TPE
 import Cedar.Thm.BatchedEvaluator
 import Cedar.Thm.WellTypedVerification
 import Cedar.Thm.Frontend
+import Cedar.Thm.Frontend.Authorizer
